[WIP] Initial work on blockverification for byte-addressing RISC-V PMP

case_study/RiscvPmpBoundedInts/BlockVer/Spec.v
@@ -42,11 +42,11 @@ From Katamaran Require Import
      Specification
      Symbolic.Executor
      Symbolic.Soundness
-     RiscvPmp.IrisModel
-     RiscvPmp.IrisInstance
-     RiscvPmp.Machine
-     RiscvPmp.Sig
-     RiscvPmp.Contracts.
+     RiscvPmpBoundedInts.IrisModel
+     RiscvPmpBoundedInts.IrisInstance
+     RiscvPmpBoundedInts.Machine
+     RiscvPmpBoundedInts.Sig
+     RiscvPmpBoundedInts.Contracts.
 
 Import RiscvPmpProgram.
 Import ListNotations.
@@ -62,18 +62,18 @@ Module Assembly.
     RTYPE rs2 rs1 rd RISCV_ADD.
   Definition SUB (rd rs1 rs2 : RegIdx) : AST :=
     RTYPE rs2 rs1 rd RISCV_SUB.
-  Definition BEQ (rs1 rs2 : RegIdx) (imm : Z) : AST :=
+  Definition BEQ (rs1 rs2 : RegIdx) (imm : bv 13) : AST :=
     BTYPE imm rs2 rs1 RISCV_BEQ.
-  Definition BNE (rs1 rs2 : RegIdx) (imm : Z) : AST :=
+  Definition BNE (rs1 rs2 : RegIdx) (imm : bv 13) : AST :=
     BTYPE imm rs2 rs1 RISCV_BNE.
-  Definition ADDI (rd rs1 : RegIdx) (imm : Z) : AST :=
+  Definition ADDI (rd rs1 : RegIdx) (imm : bv 12) : AST :=
     ITYPE imm rs1 rd RISCV_ADDI.
-  Definition JALR (rd rs1 : RegIdx) (imm : Z) : AST :=
+  Definition JALR (rd rs1 : RegIdx) (imm : bv 12) : AST :=
     RISCV_JALR imm rs1 rd.
   Definition RET : AST :=
-    JALR (bv.of_N 0) (bv.of_N 1) 0%Z.
+    JALR (bv.of_N 0) (bv.of_N 1) bv.zero.
   Definition MV (rd rs1 : RegIdx) : AST :=
-    ADDI rd rs1 0%Z.
+    ADDI rd rs1 bv.zero.
 End Assembly.
 
 Module RiscvPmpBlockVerifSpec <: Specification RiscvPmpBase RiscvPmpProgram RiscvPmpSignature.
@@ -81,8 +81,10 @@ Module RiscvPmpBlockVerifSpec <: Specification RiscvPmpBase RiscvPmpProgram Risc
   Section ContractDefKit.
 
   Import asn.notations.
-  Notation "a '↦ₘ' t" := (asn.chunk (chunk_user ptsto [a; t])) (at level 70).
-  Notation "a '↦ᵣ' t" := (asn.chunk (chunk_user ptsto_readonly [a; t])) (at level 70).
+  (* Notation "a [ bytes ]'↦ₘ' t" := (asn.chunk (chunk_user (@ptstomem bytes) [a; t])) (at level 70). *)
+  (* Notation "a [ bytes ]'↦ᵣ' t" := (asn.chunk (chunk_user (@ptstomem_readonly bytes) [a; t])) (at level 70). *)
+  Notation "a '↦ₘ' t" := (asn.chunk (chunk_user (@ptstomem bytes_per_word) [a; t])) (at level 70).
+  Notation "a '↦ᵣ' t" := (asn.chunk (chunk_user (@ptstomem_readonly bytes_per_word) [a; t])) (at level 70).
   Notation "a '↦ᵢ' t" := (asn.chunk (chunk_user ptstoinstr [a; t])) (at level 70).
   Notation "a <ₜ b" := (term_binop bop.lt a b) (at level 60).
   Notation "a <=ₜ b" := (term_binop bop.le a b) (at level 60).
@@ -92,7 +94,7 @@ Module RiscvPmpBlockVerifSpec <: Specification RiscvPmpBase RiscvPmpProgram Risc
   Notation asn_pmp_entries l := (asn.chunk (chunk_user pmp_entries [l])).
   Notation asn_pmp_all_entries_unlocked l := (asn.formula (formula_user pmp_all_entries_unlocked [l])).
   Notation asn_pmp_addr_access l m := (asn.chunk (chunk_user pmp_addr_access [l; m])).
-  Notation asn_pmp_access addr es m p := (asn.formula (formula_user pmp_access [addr;es;m;p])).
+  Notation asn_pmp_access addr width es m p := (asn.formula (formula_user pmp_access [addr;width;es;m;p])).
 
   Definition term_eqb {Σ} (e1 e2 : Term Σ ty_regno) : Term Σ ty.bool :=
     term_binop (bop.relop bop.eq) e1 e2.
@@ -141,7 +143,7 @@ Module RiscvPmpBlockVerifSpec <: Specification RiscvPmpBase RiscvPmpProgram Risc
      ⊥))))))).
 
   Definition asn_reg_ptsto {Σ} (r : Term Σ ty_regno) (w : Term Σ ty_word) : Assertion Σ :=
-    asn_with_reg r (fun r => asn.chunk (chunk_ptsreg r w)) (w = term_val ty_word 0%Z).
+    asn_with_reg r (fun r => asn.chunk (chunk_ptsreg r w)) (w = term_val ty_word bv.zero).
 
   Local Notation "e1 ',ₜ' e2" := (term_binop bop.pair e1 e2) (at level 100).
 
@@ -161,8 +163,8 @@ Module RiscvPmpBlockVerifSpec <: Specification RiscvPmpBase RiscvPmpProgram Risc
      asn.notations. Resolve this.
    *)
   Local Notation "r '↦' val" := (asn_reg_ptsto r val) : asn_scope.
-  Local Notation "a '↦ₘ' t" := (asn.chunk (chunk_user ptsto [a; t])) (at level 70).
-  Local Notation "a '↦ᵣ' t" := (asn.chunk (chunk_user ptsto_readonly [a; t])) (at level 70).
+  Local Notation "a '↦ₘ' t" := (asn.chunk (chunk_user (@ptstomem bytes_per_word) [a; t])) (at level 70).
+  Local Notation "a '↦ᵣ' t" := (asn.chunk (chunk_user (@ptstomem_readonly bytes_per_word) [a; t])) (at level 70).
   Local Notation "a '↦ᵢ' t" := (asn.chunk (chunk_user ptstoinstr [a; t])) (at level 70).
   Local Notation "a <ₜ b" := (term_binop bop.lt a b) (at level 60).
   Local Notation "a <=ₜ b" := (term_binop bop.le a b) (at level 60).
@@ -195,7 +197,7 @@ Module RiscvPmpBlockVerifSpec <: Specification RiscvPmpBase RiscvPmpProgram Risc
        sep_contract_result          := "result_wX";
        sep_contract_postcondition   := term_var "result_wX" = term_val ty.unit tt ∗
                                        if: term_eqb (term_var "rs") (term_val ty_regno [bv 0])
-                                       then term_var "rs" ↦ term_val ty_word 0%Z
+                                       then term_var "rs" ↦ term_val ty_word bv.zero
                                        else term_var "rs" ↦ term_var "v"
     |}.
 
@@ -215,8 +217,8 @@ Module RiscvPmpBlockVerifSpec <: Specification RiscvPmpBase RiscvPmpProgram Risc
        sep_contract_localstore      := [];
        sep_contract_precondition    := asn.chunk (chunk_ptsreg pc (term_var "a")) ∗
                                                  term_var "a" ↦ᵢ term_var "i" ∗
-                                                 term_val ty_xlenbits minAddr <= term_var "a" ∗
-                                                 term_var "a" <= term_val ty_xlenbits maxAddr ∗
+                                                 (term_val ty_xlenbits minAddr <=ᵘ term_var "a")%asn ∗
+                                                 (term_var "a" <=ᵘ term_val ty_xlenbits maxAddr)%asn ∗
                                                  asn_cur_privilege (term_val ty_privilege Machine) ∗
                                                  asn_pmp_entries (term_var "entries") ∗
                                                  asn_pmp_all_entries_unlocked (term_var "entries");
@@ -238,17 +240,17 @@ Module RiscvPmpBlockVerifSpec <: Specification RiscvPmpBase RiscvPmpProgram Risc
        sep_contract_postcondition   := term_var "result_pmpLocked" = term_val ty.bool false;
     |}.
 
-  Definition sep_contract_checked_mem_read : SepContractFun checked_mem_read :=
-    {| sep_contract_logic_variables := ["inv" :: ty.bool; "typ" :: ty_access_type; "paddr" :: ty_xlenbits; "w" :: ty_xlenbits];
+  Definition sep_contract_checked_mem_read {bytes} : SepContractFun (@checked_mem_read bytes) :=
+    {| sep_contract_logic_variables := ["inv" :: ty.bool; "typ" :: ty_access_type; "paddr" :: ty_xlenbits; "w" :: ty_bytes bytes];
       sep_contract_localstore      := [term_var "typ"; term_var "paddr"];
       sep_contract_precondition    :=
-        asn.match_bool (term_var "inv") (term_var "paddr" ↦ᵣ term_var "w") (term_var "paddr" ↦ₘ term_var "w") ∗
-          term_val ty_xlenbits minAddr <= term_var "paddr" ∗
-          term_var "paddr" <= term_val ty_xlenbits maxAddr;
+        asn.match_bool (term_var "inv") (asn.chunk (chunk_user (ptstomem_readonly bytes) [term_var "paddr"; term_var "w"])) (asn.chunk (chunk_user (ptstomem bytes) [term_var "paddr"; term_var "w"])) ∗
+          (term_val ty_xlenbits minAddr <=ᵘ term_var "paddr")%asn ∗
+          (term_var "paddr" <=ᵘ term_val ty_xlenbits maxAddr)%asn;
       sep_contract_result          := "result_mem_read";
       sep_contract_postcondition   :=
-        term_var "result_mem_read" = term_union memory_op_result KMemValue (term_var "w") ∗
-                                       asn.match_bool (term_var "inv") (term_var "paddr" ↦ᵣ term_var "w") (term_var "paddr" ↦ₘ term_var "w");
+        term_var "result_mem_read" = term_union (memory_op_result bytes) KMemValue (term_var "w") ∗
+                                       asn.match_bool (term_var "inv") (asn.chunk (chunk_user (ptstomem_readonly bytes) [term_var "paddr"; term_var "w"])) (asn.chunk (chunk_user (ptstomem bytes) [term_var "paddr"; term_var "w"]));
     |}.
 
   Definition sep_contract_pmpCheckPerms : SepContractFun pmpCheckPerms :=
@@ -258,13 +260,13 @@ Module RiscvPmpBlockVerifSpec <: Specification RiscvPmpBase RiscvPmpProgram Risc
          term_var "priv" = term_val ty_privilege Machine
          ∗ asn_pmp_cfg_unlocked (term_var "entry");
        sep_contract_result          := "result_pmpCheckPerms";
-       sep_contract_postcondition   := 
+       sep_contract_postcondition   :=
          term_var "result_pmpCheckPerms" = term_val ty.bool true;
     |}.
 
   Definition sep_contract_pmpMatchAddr : SepContractFun pmpMatchAddr :=
-    {| sep_contract_logic_variables := ["addr" :: ty_xlenbits; "rng" :: ty_pmp_addr_range];
-       sep_contract_localstore      := [term_var "addr"; term_var "rng"];
+    {| sep_contract_logic_variables := ["addr" :: ty_xlenbits; "width" :: ty_xlenbits; "rng" :: ty_pmp_addr_range];
+       sep_contract_localstore      := [term_var "addr"; term_var "width"; term_var "rng"];
        sep_contract_precondition    := ⊤;
        sep_contract_result          := "result_pmpMatchAddr";
        sep_contract_postcondition   :=
@@ -273,53 +275,55 @@ Module RiscvPmpBlockVerifSpec <: Specification RiscvPmpBase RiscvPmpProgram Risc
     |}.
 
   Definition sep_contract_pmpCheck : SepContractFun pmpCheck :=
-    {| sep_contract_logic_variables := ["addr" :: ty_xlenbits; "acc" :: ty_access_type; "priv" :: ty_privilege; "entries" :: ty.list ty_pmpentry];
-       sep_contract_localstore      := [term_var "addr"; term_var "acc"; term_var "priv"];
+    {| sep_contract_logic_variables := ["addr" :: ty_xlenbits; "width" :: ty_xlenbits; "acc" :: ty_access_type; "priv" :: ty_privilege; "entries" :: ty.list ty_pmpentry];
+       sep_contract_localstore      := [term_var "addr"; term_var "width"; term_var "acc"; term_var "priv"];
        sep_contract_precondition    :=
          asn_pmp_entries (term_var "entries")
          ∗ term_var "priv" = term_val ty_privilege Machine
          ∗ asn_pmp_all_entries_unlocked (term_var "entries");
        sep_contract_result          := "result_pmpCheck";
-       sep_contract_postcondition   := 
+       sep_contract_postcondition   :=
          term_var "result_pmpCheck" = term_inr (term_val ty.unit tt)
          ∗ asn_pmp_entries (term_var "entries")
-         ∗ asn_pmp_access (term_var "addr") (term_var "entries") (term_var "priv") (term_var "acc");
+         ∗ asn.formula (formula_user pmp_access [(term_var "addr"); (term_var "width"); (term_var "entries"); (term_var "priv"); (term_var "acc")])
+         (* not sure why this notation doesn't type check *)
+         (* ∗ asn_pmp_access (term_var "addr") (term_var "width") (term_var "entries") (term_var "priv") (term_var "acc"); *)
     |}.
 
-  Definition sep_contract_pmp_mem_read : SepContractFun pmp_mem_read :=
-    {| sep_contract_logic_variables := ["inv" :: ty.bool; "typ" :: ty_access_type; "paddr" :: ty_xlenbits; "entries" :: ty.list ty_pmpentry; "w" :: ty_xlenbits; "m" :: ty_privilege];
+  Definition sep_contract_pmp_mem_read {bytes} : SepContractFun (pmp_mem_read bytes) :=
+    {| sep_contract_logic_variables := ["inv" :: ty.bool; "typ" :: ty_access_type; "paddr" :: ty_xlenbits; "entries" :: ty.list ty_pmpentry; "w" :: ty_bytes bytes; "m" :: ty_privilege];
       sep_contract_localstore      := [term_var "typ"; term_var "m"; term_var "paddr"];
       sep_contract_precondition    :=
-        asn.match_bool (term_var "inv") (term_var "paddr" ↦ᵣ term_var "w") (term_var "paddr" ↦ₘ term_var "w") ∗
+        asn.match_bool (term_var "inv") (asn.chunk (chunk_user (ptstomem_readonly bytes) [term_var "paddr"; term_var "w"])) (asn.chunk (chunk_user (ptstomem bytes) [term_var "paddr"; term_var "w"])) ∗
           term_var "m" = term_val ty_privilege Machine ∗
-          term_val ty_xlenbits minAddr <= term_var "paddr" ∗
-          term_var "paddr" <= term_val ty_xlenbits maxAddr ∗
+          (term_val ty_xlenbits minAddr <=ᵘ term_var "paddr")%asn ∗
+          (term_var "paddr" <=ᵘ term_val ty_xlenbits maxAddr)%asn ∗
           asn_cur_privilege (term_val ty_privilege Machine) ∗
           asn_pmp_entries (term_var "entries") ∗
           asn_pmp_all_entries_unlocked (term_var "entries");
       sep_contract_result          := "result_mem_read";
       sep_contract_postcondition   :=
-        term_var "result_mem_read" = term_union memory_op_result KMemValue (term_var "w") ∗
-                                       asn.match_bool (term_var "inv") (term_var "paddr" ↦ᵣ term_var "w") (term_var "paddr" ↦ₘ term_var "w") ∗
+        term_var "result_mem_read" = term_union (memory_op_result bytes) KMemValue (term_var "w") ∗
+                                       asn.match_bool (term_var "inv") (asn.chunk (chunk_user (ptstomem_readonly bytes) [term_var "paddr"; term_var "w"])) (asn.chunk (chunk_user (ptstomem bytes) [term_var "paddr"; term_var "w"])) ∗
           asn_cur_privilege (term_val ty_privilege Machine) ∗
           asn_pmp_entries (term_var "entries") ∗
           asn_pmp_all_entries_unlocked (term_var "entries");
     |}.
 
-  Definition sep_contract_mem_read : SepContractFun mem_read :=
-    {| sep_contract_logic_variables := ["inv" :: ty.bool; "typ" :: ty_access_type; "paddr" :: ty_xlenbits; "entries" :: ty.list ty_pmpentry; "w" :: ty_xlenbits];
+  Definition sep_contract_mem_read {bytes} : SepContractFun (mem_read bytes) :=
+    {| sep_contract_logic_variables := ["inv" :: ty.bool; "typ" :: ty_access_type; "paddr" :: ty_xlenbits; "entries" :: ty.list ty_pmpentry; "w" :: ty_bytes bytes];
       sep_contract_localstore      := [term_var "typ"; term_var "paddr"];
       sep_contract_precondition    :=
-        asn.match_bool (term_var "inv") (term_var "paddr" ↦ᵣ term_var "w") (term_var "paddr" ↦ₘ term_var "w") ∗
-          term_val ty_xlenbits minAddr <= term_var "paddr" ∗
-          term_var "paddr" <= term_val ty_xlenbits maxAddr ∗
+        asn.match_bool (term_var "inv") (asn.chunk (chunk_user (ptstomem_readonly bytes) [term_var "paddr"; term_var "w"])) (asn.chunk (chunk_user (ptstomem bytes) [term_var "paddr"; term_var "w"])) ∗
+          (term_val ty_xlenbits minAddr <=ᵘ term_var "paddr")%asn ∗
+          (term_var "paddr" <=ᵘ term_val ty_xlenbits maxAddr)%asn ∗
           asn_cur_privilege (term_val ty_privilege Machine) ∗
           asn_pmp_entries (term_var "entries") ∗
           asn_pmp_all_entries_unlocked (term_var "entries");
       sep_contract_result          := "result_mem_read";
       sep_contract_postcondition   :=
-        term_var "result_mem_read" = term_union memory_op_result KMemValue (term_var "w") ∗
-                                       asn.match_bool (term_var "inv") (term_var "paddr" ↦ᵣ term_var "w") (term_var "paddr" ↦ₘ term_var "w") ∗
+        term_var "result_mem_read" = term_union (memory_op_result bytes) KMemValue (term_var "w") ∗
+                                       asn.match_bool (term_var "inv") (asn.chunk (chunk_user (ptstomem_readonly bytes) [term_var "paddr"; term_var "w"])) (asn.chunk (chunk_user (ptstomem bytes) [term_var "paddr"; term_var "w"])) ∗
           asn_cur_privilege (term_val ty_privilege Machine) ∗
           asn_pmp_entries (term_var "entries") ∗
           asn_pmp_all_entries_unlocked (term_var "entries");
@@ -339,19 +343,19 @@ Module RiscvPmpBlockVerifSpec <: Specification RiscvPmpBase RiscvPmpProgram Risc
   Definition CEnv : SepContractEnv :=
     fun Δ τ f =>
       match f with
-      | rX               => Some sep_contract_rX
-      | wX               => Some sep_contract_wX
-      | fetch            => Some sep_contract_fetch_instr
-      | mem_read         => Some sep_contract_mem_read
-      | tick_pc          => Some sep_contract_tick_pc
-      | pmpCheck         => Some sep_contract_pmpCheck
-      | pmpCheckPerms    => Some sep_contract_pmpCheckPerms
-      | within_phys_mem  => Some sep_contract_within_phys_mem
-      | pmpLocked        => Some sep_contract_pmpLocked
-      | pmpMatchAddr     => Some sep_contract_pmpMatchAddr
-      | pmp_mem_read     => Some sep_contract_pmp_mem_read
-      | checked_mem_read => Some sep_contract_checked_mem_read
-      | _                => None
+      | rX                     => Some sep_contract_rX
+      | wX                     => Some sep_contract_wX
+      | fetch                  => Some sep_contract_fetch_instr
+      | mem_read bytes         => Some sep_contract_mem_read
+      | tick_pc                => Some sep_contract_tick_pc
+      | pmpCheck               => Some sep_contract_pmpCheck
+      | pmpCheckPerms          => Some sep_contract_pmpCheckPerms
+      | within_phys_mem        => Some sep_contract_within_phys_mem
+      | pmpLocked              => Some sep_contract_pmpLocked
+      | pmpMatchAddr           => Some sep_contract_pmpMatchAddr
+      | pmp_mem_read bytes     => Some sep_contract_pmp_mem_read
+      | checked_mem_read bytes => Some sep_contract_checked_mem_read
+      | _                      => None
       end.
 
   Lemma linted_cenv :
@@ -362,24 +366,24 @@ Module RiscvPmpBlockVerifSpec <: Specification RiscvPmpBase RiscvPmpProgram Risc
       end.
   Proof. intros ? ? []; try constructor. Qed.
 
-  Definition sep_contract_read_ram : SepContractFunX read_ram :=
-    {| sep_contract_logic_variables := ["inv" :: ty.bool; "paddr" :: ty_xlenbits; "w" :: ty_xlenbits];
+  Definition sep_contract_read_ram {bytes} : SepContractFunX (read_ram bytes) :=
+    {| sep_contract_logic_variables := ["inv" :: ty.bool; "paddr" :: ty_xlenbits; "w" :: ty_bytes bytes];
        sep_contract_localstore      := [term_var "paddr"];
-       sep_contract_precondition    := asn.match_bool (term_var "inv") (term_var "paddr" ↦ᵣ term_var "w") (term_var "paddr" ↦ₘ term_var "w");
+       sep_contract_precondition    := asn.match_bool (term_var "inv") (asn.chunk (chunk_user (ptstomem_readonly bytes) [term_var "paddr"; term_var "w"])) (asn.chunk (chunk_user (ptstomem bytes) [term_var "paddr"; term_var "w"]));
        sep_contract_result          := "result_read_ram";
        sep_contract_postcondition   := asn.match_bool (term_var "inv")
-                                         (term_var "paddr" ↦ᵣ term_var "w")
-                                         (term_var "paddr" ↦ₘ term_var "w") ∗
+                                         (asn.chunk (chunk_user (ptstomem_readonly bytes) [term_var "paddr"; term_var "w"]))
+                                         (asn.chunk (chunk_user (ptstomem bytes) [term_var "paddr"; term_var "w"])) ∗
                                             term_var "result_read_ram" = term_var "w";
     |}.
 
-  Definition sep_contract_write_ram : SepContractFunX write_ram :=
-    {| sep_contract_logic_variables := ["paddr" :: ty_word; "data" :: ty_word];
+  Definition sep_contract_write_ram {bytes} : SepContractFunX (write_ram bytes) :=
+    {| sep_contract_logic_variables := ["paddr" :: ty_word; "data" :: ty_bytes bytes];
        sep_contract_localstore      := [term_var "paddr"; term_var "data"];
-       sep_contract_precondition    := ∃ "w", (term_var "paddr" ↦ₘ term_var "w");
+       sep_contract_precondition    := ∃ "w", (asn.chunk (chunk_user (ptstomem bytes) [term_var "paddr"; term_var "w"]));
        sep_contract_result          := "result_write_ram";
-       sep_contract_postcondition   := term_var "paddr" ↦ₘ term_var "data" ∗
-                                       term_var "result_write_ram" = term_val ty_word 1%Z;
+       sep_contract_postcondition   := (asn.chunk (chunk_user (ptstomem bytes) [term_var "paddr"; term_var "data"])) ∗
+                                       term_var "result_write_ram" = term_val ty.bool true;
     |}.
 
   Definition sep_contract_decode    : SepContractFunX decode :=
@@ -393,8 +397,8 @@ Module RiscvPmpBlockVerifSpec <: Specification RiscvPmpBase RiscvPmpProgram Risc
   Definition CEnvEx : SepContractEnvEx :=
     fun Δ τ f =>
       match f with
-      | read_ram  => sep_contract_read_ram
-      | write_ram => sep_contract_write_ram
+      | read_ram bytes  => sep_contract_read_ram
+      | write_ram bytes => sep_contract_write_ram
       | decode    => sep_contract_decode
       end.
 
@@ -423,14 +427,14 @@ Module RiscvPmpBlockVerifSpec <: Specification RiscvPmpBase RiscvPmpProgram Risc
     {| lemma_logic_variables := ["paddr" :: ty_word; "i" :: ty_ast];
        lemma_patterns        := [term_var "paddr"];
        lemma_precondition    := asn.chunk (chunk_user ptstoinstr [term_var "paddr"; term_var "i"]);
-      lemma_postcondition   := ∃ "w", (asn.chunk (chunk_user ptsto [term_var "paddr"; term_var "w"]) ∗
+      lemma_postcondition   := ∃ "w", (asn.chunk (chunk_user (ptstomem bytes_per_word) [term_var "paddr"; term_var "w"]) ∗
                                       asn.chunk (chunk_user encodes_instr [term_var "w"; term_var "i"]))
     |}.
 
   Definition lemma_close_ptsto_instr : SepLemma close_ptsto_instr :=
     {| lemma_logic_variables := ["paddr" :: ty_word; "w" :: ty_word; "i" :: ty_ast];
        lemma_patterns        := [term_var "paddr"; term_var "w"];
-       lemma_precondition    := asn.chunk (chunk_user ptsto [term_var "paddr"; term_var "w"]) ∗
+       lemma_precondition    := asn.chunk (chunk_user (ptstomem bytes_per_word) [term_var "paddr"; term_var "w"]) ∗
                                   asn.chunk (chunk_user encodes_instr [term_var "w"; term_var "i"]);
        lemma_postcondition   := asn.chunk (chunk_user ptstoinstr [term_var "paddr"; term_var "i"]);
     |}.
@@ -449,14 +453,14 @@ Module RiscvPmpBlockVerifSpec <: Specification RiscvPmpBase RiscvPmpProgram Risc
        lemma_postcondition   := ⊤;
     |}.
 
-  Definition lemma_extract_pmp_ptsto : SepLemma extract_pmp_ptsto :=
+  Definition lemma_extract_pmp_ptsto bytes : SepLemma (extract_pmp_ptsto bytes) :=
     {| lemma_logic_variables := ["paddr" :: ty_xlenbits];
        lemma_patterns        := [term_var "paddr"];
        lemma_precondition    := ⊤;
        lemma_postcondition   := ⊤;
     |}.
 
-  Definition lemma_return_pmp_ptsto : SepLemma return_pmp_ptsto :=
+  Definition lemma_return_pmp_ptsto bytes : SepLemma (return_pmp_ptsto bytes) :=
     {| lemma_logic_variables := ["paddr" :: ty_xlenbits];
        lemma_patterns        := [term_var "paddr"];
        lemma_precondition    := ⊤;
@@ -472,8 +476,8 @@ Module RiscvPmpBlockVerifSpec <: Specification RiscvPmpBase RiscvPmpProgram Risc
        | close_ptsto_instr     => lemma_close_ptsto_instr
        | open_pmp_entries                   => lemma_machine_unlocked_open_pmp_entries
        | close_pmp_entries                  => lemma_machine_unlocked_close_pmp_entries
-       | extract_pmp_ptsto => lemma_extract_pmp_ptsto
-       | return_pmp_ptsto => lemma_return_pmp_ptsto
+       | extract_pmp_ptsto bytes => lemma_extract_pmp_ptsto bytes
+       | return_pmp_ptsto bytes => lemma_return_pmp_ptsto bytes
       end.
 End RiscvPmpBlockVerifSpec.
 
@@ -547,81 +551,94 @@ Module RiscvPmpSpecVerif.
   Lemma valid_pmpLocked : ValidContract pmpLocked.
   Proof. now compute. Qed.
 
-  Lemma valid_checked_mem_read : ValidContractDebug checked_mem_read.
+  Lemma valid_checked_mem_read {bytes} : ValidContractDebug (checked_mem_read bytes).
   Proof.
     (* strange: replacing ValidContractDebug with ValidContract makes the proof fail. *)
-    symbolic_simpl.
-    now intuition.
-  Qed.
+  Admitted.
+  (*   symbolic_simpl. *)
+  (*   intuition. *)
+  (* Qed. *)
 
-  Lemma valid_pmp_mem_read : ValidContract pmp_mem_read.
-  Proof. reflexivity. Qed.
+  Lemma valid_pmp_mem_read {bytes} : ValidContract (pmp_mem_read bytes).
+  Admitted.
+  (* Proof. reflexivity. Qed. *)
 
   Lemma valid_pmpMatchAddr : ValidContractDebug pmpMatchAddr.
-  Proof. symbolic_simpl. intros. Lia.lia. Qed.
+  Proof. symbolic_simpl. intros.
+  Admitted.
+ (* Lia.lia. Qed. *)
 
   Lemma valid_pmpCheckPerms : ValidContract pmpCheckPerms.
   Proof. reflexivity. Qed.
 
   (* TODO: a lot of the following lemmas are copied from the Model, they are only used here, so omit them from the Model? *)
   (* TODO: we will never have a partial match because we are using integers instead of bitvectors, eventually this lemma will make no sense *)
-  Lemma pmp_match_addr_never_partial : forall (a : Xlenbits) (rng : PmpAddrRange),
-      pmp_match_addr a rng = PMP_Match \/ pmp_match_addr a rng = PMP_NoMatch.
+  Lemma pmp_match_addr_never_partial : forall (a : Xlenbits) width (rng : PmpAddrRange),
+      pmp_match_addr a width rng = PMP_Match \/ pmp_match_addr a width rng = PMP_NoMatch.
   Proof.
-    intros a [[lo hi]|]; cbn;
+    intros a width [[lo hi]|]; cbn;
       repeat
         match goal with
         | |- context[Z.leb ?x ?y] => destruct (Z.leb_spec x y); cbn
         | |- context[Z.ltb ?x ?y] => destruct (Z.ltb_spec x y); cbn
-        end; auto; Lia.lia.
-  Qed.
+        end; auto.
+  Admitted.
+  (* Lia.lia. *)
+  (* Qed. *)
 
-  Lemma machine_unlocked_check_pmp_access : forall (cfg0 cfg1 : Pmpcfg_ent) (a0 a1 addr : Xlenbits),
+  Lemma machine_unlocked_check_pmp_access : forall width (cfg0 cfg1 : Pmpcfg_ent) (a0 a1 addr : Xlenbits),
       Pmp_cfg_unlocked cfg0 /\ Pmp_cfg_unlocked cfg1 ->
-      check_pmp_access addr [(cfg0, a0); (cfg1, a1)]%list Machine = (true, None) \/ check_pmp_access addr [(cfg0, a0); (cfg1, a1)]%list Machine = (true, Some PmpRWX).
+      check_pmp_access addr width [(cfg0, a0); (cfg1, a1)]%list Machine = (true, None) \/ check_pmp_access addr width [(cfg0, a0); (cfg1, a1)]%list Machine = (true, Some PmpRWX).
   Proof.
     intros cfg0 cfg1 a0 a1 addr [Hcfg0 Hcfg1].
     unfold check_pmp_access, pmp_check.
     unfold pmp_match_entry.
-    apply Pmp_cfg_unlocked_bool in Hcfg0.
-    apply Pmp_cfg_unlocked_bool in Hcfg1.
-    destruct (pmp_match_addr_never_partial addr (pmp_addr_range cfg1 a1 a0)) as [-> | ->];
-      destruct (pmp_match_addr_never_partial addr (pmp_addr_range cfg0 a0 0%Z)) as [-> | ->];
-      unfold pmp_get_perms;
-      rewrite ?Hcfg0, ?Hcfg1;
-      auto.
-  Qed.
+  Admitted.
+  (*   apply Pmp_cfg_unlocked_bool in Hcfg0. *)
+  (*   apply Pmp_cfg_unlocked_bool in Hcfg1. *)
+  (*   destruct (pmp_match_addr_never_partial addr (pmp_addr_range cfg1 a1 a0)) as [-> | ->]; *)
+  (*     destruct (pmp_match_addr_never_partial addr (pmp_addr_range cfg0 a0 0%Z)) as [-> | ->]; *)
+  (*     unfold pmp_get_perms; *)
+  (*     rewrite ?Hcfg0, ?Hcfg1; *)
+  (*     auto. *)
+  (* Qed. *)
 
-  Lemma machine_unlocked_pmp_access : forall (addr : Val ty_xlenbits) (cfg0 cfg1 : Val ty_pmpcfg_ent) (a0 a1 : Val ty_xlenbits) (acc : Val ty_access_type),
+  Lemma machine_unlocked_pmp_access : forall width (addr : Val ty_xlenbits) (cfg0 cfg1 : Val ty_pmpcfg_ent) (a0 a1 : Val ty_xlenbits) (acc : Val ty_access_type),
       Pmp_cfg_unlocked cfg0 /\ Pmp_cfg_unlocked cfg1 ->
-      Pmp_access addr [(cfg0, a0); (cfg1, a1)]%list Machine acc.
+      Pmp_access addr width [(cfg0, a0); (cfg1, a1)]%list Machine acc.
   Proof.
     intros.
     unfold Pmp_access, decide_pmp_access.
-    destruct (machine_unlocked_check_pmp_access a0 a1 addr H) as [|].
-    - destruct (check_pmp_access addr _ Machine).
-      now inversion H0.
-    - destruct (check_pmp_access addr _ Machine).
-      inversion H0.
-      unfold decide_access_pmp_perm; destruct acc; auto.
-  Qed.
+  Admitted.
+  (*   destruct (machine_unlocked_check_pmp_access a0 a1 addr H) as [|]. *)
+  (*   - destruct (check_pmp_access addr _ Machine). *)
+  (*     now inversion H0. *)
+  (*   - destruct (check_pmp_access addr _ Machine). *)
+  (*     inversion H0. *)
+  (*     unfold decide_access_pmp_perm; destruct acc; auto. *)
+  (* Qed. *)
 
   Lemma valid_pmpCheck : ValidContractWithFuelDebug 3 pmpCheck.
   Proof.
     hnf. apply verification_condition_with_erasure_sound. vm_compute.
     constructor. cbn.
     intros; subst.
-    repeat try split; subst; unfold Pmp_entry_unlocked, Pmp_cfg_unlocked in *;
-    rewrite ?is_pmp_cfg_unlocked_bool in *; cbn in *; subst; try reflexivity;
-    apply machine_unlocked_pmp_access;
-      now cbn.
-  Qed.
+  Admitted.
+  (*   repeat try split; subst; unfold Pmp_entry_unlocked, Pmp_cfg_unlocked in *; *)
+  (*   rewrite ?is_pmp_cfg_unlocked_bool in *; cbn in *; subst; try reflexivity; *)
+  (*   apply machine_unlocked_pmp_access; *)
+  (*     now cbn. *)
+  (* Qed. *)
 
-  Lemma valid_mem_read : ValidContract mem_read.
-  Proof. reflexivity. Qed.
+  Lemma valid_mem_read {bytes} : ValidContract (mem_read bytes).
+  Proof.
+  Admitted.
+ (* reflexivity. Qed. *)
 
   Lemma valid_contract_within_phys_mem : ValidContractDebug within_phys_mem.
-  Proof. symbolic_simpl. intros. Lia.lia. Qed.
+  Proof. symbolic_simpl. intros.
+  Admitted.
+  (* Lia.lia. Qed. *)
 
   Lemma valid_contract : forall {Δ τ} (f : Fun Δ τ) (c : SepContract Δ τ),
       RiscvPmpBlockVerifSpec.CEnv f = Some c ->
@@ -698,8 +715,8 @@ Module RiscvPmpIrisInstanceWithContracts.
   Import iris.proofmode.string_ident.
   Import iris.proofmode.tactics.
 
-  Lemma read_ram_sound `{sailGS Σ} :
-    ValidContractForeign RiscvPmpBlockVerifSpec.sep_contract_read_ram read_ram.
+  Lemma read_ram_sound `{sailGS Σ} {bytes} :
+    ValidContractForeign RiscvPmpBlockVerifSpec.sep_contract_read_ram (read_ram bytes).
   Proof.
     intros Γ es δ ι Heq.
     destruct (env.view ι) as [ι w].
@@ -712,66 +729,67 @@ Module RiscvPmpIrisInstanceWithContracts.
     iDestruct "Hmem" as (memmap) "[Hmem' %]".
     destruct b; cbn.
     - iDestruct "ptsto_addr_w" as "#ptsto_addr_w".
-      unfold interp_ptsto_readonly.
-      iInv "ptsto_addr_w" as "Hptsto" "Hclose_ptsto".
-      iMod (fupd_mask_subseteq empty) as "Hclose_rest"; first set_solver.
-      iModIntro.
-      iSplitR; first done.
-      iIntros (e2 σ'' efs Hstep).
-      dependent elimination Hstep.
-      fold_semWP.
-      dependent elimination s.
-      rewrite Heq in f1. cbv in f1.
-      dependent elimination f1. cbn.
-      do 3 iModIntro.
-      unfold interp_ptsto.
-      iAssert (⌜ memmap !! paddr = Some w ⌝)%I with "[Hptsto Hmem']" as "%".
-      { iApply (gen_heap.gen_heap_valid with "Hmem' Hptsto"). }
-      iMod "Hclose_rest" as "_".
-      iMod ("Hclose_ptsto" with "Hptsto") as "_".
-      iModIntro.
-      iSplitL "Hmem' Hregs".
-      iSplitL "Hregs"; first iFrame.
-      iExists memmap.
-      iSplitL "Hmem'"; first iFrame.
-      iPureIntro; assumption.
-      iSplitL; last easy.
-      apply map_Forall_lookup_1 with (i := paddr) (x := w) in H0; auto.
-      cbn in H0. subst.
-      iApply wp_value.
-      iSplitL; last easy.
-      now iSplitL.
-    - iMod (fupd_mask_subseteq empty) as "Hclose"; first set_solver.
-      iModIntro.
-      iSplitR; first easy.
-      iIntros (e2 σ'' efs Hstep).
-      dependent elimination Hstep.
-      fold_semWP.
-      dependent elimination s.
-      rewrite Heq in f1. cbv in f1.
-      dependent elimination f1. cbn.
-      do 3 iModIntro.
-      unfold interp_ptsto.
-      iAssert (⌜ memmap !! paddr = Some w ⌝)%I with "[ptsto_addr_w Hmem']" as "%".
-      { iApply (gen_heap.gen_heap_valid with "Hmem' ptsto_addr_w"). }
-      iMod "Hclose" as "_".
-      iModIntro.
-      iSplitL "Hmem' Hregs".
-      iSplitL "Hregs"; first iFrame.
-      iExists memmap.
-      iSplitL "Hmem'"; first iFrame.
-      iPureIntro; assumption.
-      iSplitL; last easy.
-      apply map_Forall_lookup_1 with (i := paddr) (x := w) in H0; auto.
-      cbn in H0. subst.
-      iApply wp_value.
-      iSplitL; last easy.
-      iSplitL; last easy.
-      iAssumption.
-  Qed.
+  (*     unfold interp_ptsto_readonly. *)
+  (*     iInv "ptsto_addr_w" as "Hptsto" "Hclose_ptsto". *)
+  (*     iMod (fupd_mask_subseteq empty) as "Hclose_rest"; first set_solver. *)
+  (*     iModIntro. *)
+  (*     iSplitR; first done. *)
+  (*     iIntros (e2 σ'' efs Hstep). *)
+  (*     dependent elimination Hstep. *)
+  (*     fold_semWP. *)
+  (*     dependent elimination s. *)
+  (*     rewrite Heq in f1. cbv in f1. *)
+  (*     dependent elimination f1. cbn. *)
+  (*     do 3 iModIntro. *)
+  (*     unfold interp_ptsto. *)
+  (*     iAssert (⌜ memmap !! paddr = Some w ⌝)%I with "[Hptsto Hmem']" as "%". *)
+  (*     { iApply (gen_heap.gen_heap_valid with "Hmem' Hptsto"). } *)
+  (*     iMod "Hclose_rest" as "_". *)
+  (*     iMod ("Hclose_ptsto" with "Hptsto") as "_". *)
+  (*     iModIntro. *)
+  (*     iSplitL "Hmem' Hregs". *)
+  (*     iSplitL "Hregs"; first iFrame. *)
+  (*     iExists memmap. *)
+  (*     iSplitL "Hmem'"; first iFrame. *)
+  (*     iPureIntro; assumption. *)
+  (*     iSplitL; last easy. *)
+  (*     apply map_Forall_lookup_1 with (i := paddr) (x := w) in H0; auto. *)
+  (*     cbn in H0. subst. *)
+  (*     iApply wp_value. *)
+  (*     iSplitL; last easy. *)
+  (*     now iSplitL. *)
+  (*   - iMod (fupd_mask_subseteq empty) as "Hclose"; first set_solver. *)
+  (*     iModIntro. *)
+  (*     iSplitR; first easy. *)
+  (*     iIntros (e2 σ'' efs Hstep). *)
+  (*     dependent elimination Hstep. *)
+  (*     fold_semWP. *)
+  (*     dependent elimination s. *)
+  (*     rewrite Heq in f1. cbv in f1. *)
+  (*     dependent elimination f1. cbn. *)
+  (*     do 3 iModIntro. *)
+  (*     unfold interp_ptsto. *)
+  (*     iAssert (⌜ memmap !! paddr = Some w ⌝)%I with "[ptsto_addr_w Hmem']" as "%". *)
+  (*     { iApply (gen_heap.gen_heap_valid with "Hmem' ptsto_addr_w"). } *)
+  (*     iMod "Hclose" as "_". *)
+  (*     iModIntro. *)
+  (*     iSplitL "Hmem' Hregs". *)
+  (*     iSplitL "Hregs"; first iFrame. *)
+  (*     iExists memmap. *)
+  (*     iSplitL "Hmem'"; first iFrame. *)
+  (*     iPureIntro; assumption. *)
+  (*     iSplitL; last easy. *)
+  (*     apply map_Forall_lookup_1 with (i := paddr) (x := w) in H0; auto. *)
+  (*     cbn in H0. subst. *)
+  (*     iApply wp_value. *)
+  (*     iSplitL; last easy. *)
+  (*     iSplitL; last easy. *)
+  (*     iAssumption. *)
+  (* Qed. *)
+  Admitted.
 
-  Lemma write_ram_sound `{sailGS Σ} :
-    ValidContractForeign RiscvPmpBlockVerifSpec.sep_contract_write_ram write_ram.
+  Lemma write_ram_sound `{sailGS Σ} {bytes} :
+    ValidContractForeign RiscvPmpBlockVerifSpec.sep_contract_write_ram (write_ram bytes).
   Proof.
     intros Γ es δ ι Heq.
     destruct (env.view ι) as [ι data].
@@ -792,27 +810,28 @@ Module RiscvPmpIrisInstanceWithContracts.
     dependent elimination f1. cbn.
     do 3 iModIntro.
     unfold interp_ptsto.
-    iMod (gen_heap.gen_heap_update _ _ _ data with "Hmem' ptsto_addr") as "[Hmem' ptsto_addr]".
-    iMod "Hclose" as "_".
-    iModIntro.
-    iSplitL "Hmem' Hregs".
-    iSplitL "Hregs"; first iFrame.
-    iExists (<[paddr:=data]> memmap).
-    iSplitL "Hmem'"; first iFrame.
-    iPureIntro.
-    { apply map_Forall_lookup.
-      intros i x Hl.
-      unfold fun_write_ram.
-      destruct (Z.eqb_spec paddr i).
-      + subst. apply (lookup_insert_rev memmap i); assumption.
-      + rewrite -> map_Forall_lookup in H0.
-        rewrite -> lookup_insert_ne in Hl; auto.
-    }
-    iSplitL; last easy.
-    iApply wp_value.
-    iSplitL; trivial.
-    iSplitL; trivial.
-  Qed.
+  (*   iMod (gen_heap.gen_heap_update _ _ _ data with "Hmem' ptsto_addr") as "[Hmem' ptsto_addr]". *)
+  (*   iMod "Hclose" as "_". *)
+  (*   iModIntro. *)
+  (*   iSplitL "Hmem' Hregs". *)
+  (*   iSplitL "Hregs"; first iFrame. *)
+  (*   iExists (<[paddr:=data]> memmap). *)
+  (*   iSplitL "Hmem'"; first iFrame. *)
+  (*   iPureIntro. *)
+  (*   { apply map_Forall_lookup. *)
+  (*     intros i x Hl. *)
+  (*     unfold fun_write_ram. *)
+  (*     destruct (Z.eqb_spec paddr i). *)
+  (*     + subst. apply (lookup_insert_rev memmap i); assumption. *)
+  (*     + rewrite -> map_Forall_lookup in H0. *)
+  (*       rewrite -> lookup_insert_ne in Hl; auto. *)
+  (*   } *)
+  (*   iSplitL; last easy. *)
+  (*   iApply wp_value. *)
+  (*   iSplitL; trivial. *)
+  (*   iSplitL; trivial. *)
+  (* Qed. *)
+  Admitted.
 
   Lemma decode_sound `{sailGS Σ} :
     ValidContractForeign RiscvPmpBlockVerifSpec.sep_contract_decode RiscvPmpProgram.decode.
@@ -894,46 +913,48 @@ Module RiscvPmpIrisInstanceWithContracts.
     destruct entries; try done.
     destruct v as [cfg1 addr1].
     destruct entries; try done.
-    iDestruct "Hunlocked" as "[[%Hcfg0 [%Hcfg1 _]] _]".
-    unfold interp_pmp_entries.
-    apply Pmp_cfg_unlocked_bool in Hcfg0.
-    apply Pmp_cfg_unlocked_bool in Hcfg1.
-    iDestruct "Hentries" as "(? & ? & ? & ?)".
-    iExists cfg0.
-    iExists addr0.
-    iExists cfg1.
-    iExists addr1.
-    iFrame.
-    now rewrite ?Pmp_cfg_unlocked_bool.
-  Qed.
+  (*   iDestruct "Hunlocked" as "[[%Hcfg0 [%Hcfg1 _]] _]". *)
+  (*   unfold interp_pmp_entries. *)
+  (*   apply Pmp_cfg_unlocked_bool in Hcfg0. *)
+  (*   apply Pmp_cfg_unlocked_bool in Hcfg1. *)
+  (*   iDestruct "Hentries" as "(? & ? & ? & ?)". *)
+  (*   iExists cfg0. *)
+  (*   iExists addr0. *)
+  (*   iExists cfg1. *)
+  (*   iExists addr1. *)
+  (*   iFrame. *)
+  (*   now rewrite ?Pmp_cfg_unlocked_bool. *)
+  (* Qed. *)
+  Admitted.
 
   Lemma machine_unlocked_close_pmp_entries_sound `{sailGS Σ} :
     ValidLemma RiscvPmpSpecification.lemma_machine_unlocked_close_pmp_entries.
   Proof.
     intros ι; destruct_syminstance ι; cbn.
     iIntros "(? & ? & ? & ? & _ & _ & [%Hunlocked0 _] & [%Hunlocked1 _])".
-    now iFrame.
-  Qed.
+  (*   now iFrame. *)
+  (* Qed. *)
+  Admitted.
 
-  Lemma in_liveAddrs_split : forall (addr : Addr),
-      (minAddr <= addr)%Z ->
-      (addr <= maxAddr)%Z ->
-      exists l1 l2, liveAddrs = l1 ++ ([addr] ++ l2).
-  Proof.
-    intros addr Hmin Hmax.
-    unfold liveAddrs.
-    exists (seqZ minAddr (addr - minAddr)).
-    exists (seqZ (addr + 1) (maxAddr - addr)).
-    transitivity (seqZ minAddr (addr - minAddr) ++ seqZ (addr) (maxAddr - addr + 1)).
-    refine (eq_trans _ (eq_trans (seqZ_app minAddr (addr - minAddr) (maxAddr - addr + 1) _ _) _));
-      do 2 (f_equal; try lia).
-    f_equal; cbn.
-    refine (eq_trans (seqZ_cons _ _ _) _); try lia.
-    do 2 f_equal; lia.
-  Qed.
+  (* Lemma in_liveAddrs_split : forall (addr : Addr), *)
+  (*     (minAddr <= addr)%Z -> *)
+  (*     (addr <= maxAddr)%Z -> *)
+  (*     exists l1 l2, liveAddrs = l1 ++ ([addr] ++ l2). *)
+  (* Proof. *)
+  (*   intros addr Hmin Hmax. *)
+  (*   unfold liveAddrs. *)
+  (*   exists (seqZ minAddr (addr - minAddr)). *)
+  (*   exists (seqZ (addr + 1) (maxAddr - addr)). *)
+  (*   transitivity (seqZ minAddr (addr - minAddr) ++ seqZ (addr) (maxAddr - addr + 1)). *)
+  (*   refine (eq_trans _ (eq_trans (seqZ_app minAddr (addr - minAddr) (maxAddr - addr + 1) _ _) _)); *)
+  (*     do 2 (f_equal; try lia). *)
+  (*   f_equal; cbn. *)
+  (*   refine (eq_trans (seqZ_cons _ _ _) _); try lia. *)
+  (*   do 2 f_equal; lia. *)
+  (* Qed. *)
 
-  Lemma extract_pmp_ptsto_sound `{sailGS Σ} :
-    ValidLemma RiscvPmpSpecification.lemma_extract_pmp_ptsto.
+  Lemma extract_pmp_ptsto_sound `{sailGS Σ} {bytes} :
+    ValidLemma (RiscvPmpSpecification.lemma_extract_pmp_ptsto bytes).
   Proof.
     intros ι; destruct_syminstance ι; cbn.
     rewrite ?Z.leb_le.
@@ -943,21 +964,22 @@ Module RiscvPmpIrisInstanceWithContracts.
       interp_ptsto,
       MemVal, Word.
 
-    destruct (in_liveAddrs_split Hlemin Hlemax) as (l1 & l2 & eq).
-    rewrite eq.
-    rewrite big_opL_app big_opL_cons.
-    iDestruct "Hmem" as "[Hmem1 [Hpaddr Hmem2]]".
-    iSplitR "Hpaddr".
-    - iIntros "Hpaddr".
-      iFrame.
-      now iIntros "_".
-    - iApply "Hpaddr".
-      iPureIntro.
-      now exists acc.
-  Qed.
+  (*   destruct (in_liveAddrs_split Hlemin Hlemax) as (l1 & l2 & eq). *)
+  (*   rewrite eq. *)
+  (*   rewrite big_opL_app big_opL_cons. *)
+  (*   iDestruct "Hmem" as "[Hmem1 [Hpaddr Hmem2]]". *)
+  (*   iSplitR "Hpaddr". *)
+  (*   - iIntros "Hpaddr". *)
+  (*     iFrame. *)
+  (*     now iIntros "_". *)
+  (*   - iApply "Hpaddr". *)
+  (*     iPureIntro. *)
+  (*     now exists acc. *)
+  (* Qed. *)
+  Admitted.
 
-  Lemma return_pmp_ptsto_sound `{sailGS Σ} :
-    ValidLemma RiscvPmpSpecification.lemma_return_pmp_ptsto.
+  Lemma return_pmp_ptsto_sound `{sailGS Σ} {bytes} :
+    ValidLemma (RiscvPmpSpecification.lemma_return_pmp_ptsto bytes).
   Proof.
     intros ι; destruct_syminstance ι; cbn.
     iIntros "[Hwithout Hptsto]".
