case_study/RiscvPmpBoundedInts/Base.v
@@ -46,10 +46,11 @@ Local Set Implicit Arguments.
 Local Notation "( x ; y )" := (existT x y) (only parsing).
 
 Definition xlen      := 32.
-Definition byte      := 8.
-Definition word      := 4 * byte.
-Definition xlenbytes := 4.
-Definition xlenbits  := xlenbytes * byte.
+Definition byte           := 8.
+Definition bytes_per_word := 4.
+Definition word           := bytes_per_word * byte.
+Definition xlenbytes      := 4.
+Definition xlenbits       := xlenbytes * byte.
 
 #[export] Instance IsTrue_bytes_xlenbytes (x y: nat) (H : IsTrue (x <=? y)): IsTrue (x * byte <=? y * byte).
 Proof.
